verified/exceptions.i.dfy
@@ -177,7 +177,7 @@ lemma lemma_svc_returning_verify_step0_helper(s:state, pagedb:PageDb, dispPg:Pag
     requires pageDbCorresponds(m1, pagedb)
     requires validDispatcherPage(pagedb, dispPg)
     requires |user_words| == 8
-    requires pagedb' == pagedb[dispPg := pagedb[dispPg].(entry := pagedb[dispPg].entry.(verifywords := user_words))]
+    requires pagedb' == pagedb[dispPg := pagedb[dispPg].(entry := pagedb[dispPg].entry.(verify_words := user_words))]
     requires disp == pagedb'[dispPg].entry
     requires ValidMemState(m2)
     requires pg == extractPage(m2, dispPg)
@@ -189,6 +189,47 @@ lemma lemma_svc_returning_verify_step0_helper(s:state, pagedb:PageDb, dispPg:Pag
     requires
         forall i :: 0 <= i < 8 ==>
             var a := page_monvaddr(dispPg) + DISP_CTXT_USER_WORDS + i * WORDSIZE;
+            a in m2.addresses && m2.addresses[a] == user_words[i]
+    ensures pageDbDispatcherCorresponds(dispPg, disp, pg)
+    ensures validDispatcherPage(pagedb', dispPg)
+{
+    assert pageDbDispatcherCorresponds(dispPg, disp, pg) by
+    {
+        reveal pageContentsCorresponds();
+        reveal pageDbDispatcherCorresponds();
+    }
+
+    assert validDispatcherPage(pagedb', dispPg) by
+    {
+        reveal validPageDb();
+        forall n | validPageNr(n) && n != dispPg && pagedb'[n].PageDbEntryTyped? && pagedb'[n].entry.Addrspace?
+            ensures validPageDbEntry(pagedb', n)
+        {
+            assert addrspaceRefs(pagedb, n) == addrspaceRefs(pagedb', n); // set equality
+        }
+    }
+}
+
+lemma lemma_svc_returning_verify_step1_helper(s:state, pagedb:PageDb, dispPg:PageNr, m1:memstate,
+    m2:memstate, user_words:seq<word>, pagedb':PageDb, disp:PageDbEntryTyped, pg:memmap)
+    requires SaneState(s);
+    requires m1 == s.m;
+    requires validPageDb(pagedb)
+    requires pageDbCorresponds(m1, pagedb)
+    requires validDispatcherPage(pagedb, dispPg)
+    requires |user_words| == 8
+    requires pagedb' == pagedb[dispPg := pagedb[dispPg].(entry := pagedb[dispPg].entry.(verify_measurement := user_words))]
+    requires disp == pagedb'[dispPg].entry
+    requires ValidMemState(m2)
+    requires pg == extractPage(m2, dispPg)
+    requires
+        forall i :: i in m1.addresses <==> i in m2.addresses
+    requires
+        forall i :: !(0 <= i - (page_monvaddr(dispPg) + DISP_CTXT_VERIFY_MEASUREMENT ) <= 7 * WORDSIZE) ==>
+            i in m1.addresses ==> m1.addresses[i] == m2.addresses[i]
+    requires
+        forall i :: 0 <= i < 8 ==>
+            var a := page_monvaddr(dispPg) + DISP_CTXT_VERIFY_MEASUREMENT + i * WORDSIZE;
             a in m2.addresses && m2.addresses[a] == user_words[i]
     ensures pageDbDispatcherCorresponds(dispPg, disp, pg)
     ensures validDispatcherPage(pagedb', dispPg)
